Revert "oops that didn't achieve anything"
This reverts commit dcd57f8c50f604f9de9544ccdc5b46d98386f2dc.

src/util/FilteredSet.v
@@ -5,33 +5,25 @@ From Stdlib Require Import List.
 Module fset.
   Class impl {T : Type} :=
     { rep : Type;
+      P : T -> bool;
       to_list : rep -> list T;
       of_list : list T -> rep;
     }.
+  Arguments impl : clear implicits.
   #[global] Hint Mode impl + : typeclass_instances.
   #[local] Hint Mode impl - : typeclass_instances.
-  Arguments impl : clear implicits.
-
-  Class ok {T P} {impl : impl T} := {
+  Class ok {T} {impl : impl T} := {
       ext : forall s1 s2, same_set (to_list s1) (to_list s2) -> s1 = s2;
       to_list_of_list : forall s, same_set (to_list (of_list s)) (filter P s);
       of_list_to_list : forall s, of_list (to_list s) = s;
     }.
-  #[global] Hint Mode ok + - + : typeclass_instances.
-  Arguments ok {_} _ _.
+  Arguments ok {_} _.
 
-  Class impls {T} := { impl_with : (T -> bool) -> impl T }.
-  #[global] Hint Mode impls + : typeclass_instances.
-  #[local] Hint Mode impls - : typeclass_instances.
-  Arguments impls : clear implicits.
-
-  Class oks {T} {impls : impls T} := { ok_with : forall P, ok P (impl_with P) }.
-  #[global] Hint Mode oks + + : typeclass_instances.
-  Arguments oks {_} _.
-  #[global] Existing Instance fset.ok_with.
+  Class impl_with {T} (P : T -> bool) := { _impl : impl T }.
+  #[global] Instance fset_with_inst {T} {i : impl T} : impl_with i.(P) := { _impl := _ }.
 
   Section __.
-    Context {T P} {impl : impl T} {ok : ok P impl}.
+    Context {T} {impl : impl T} {ok : ok impl}.
 
     Definition has s x := In x (to_list s).
 
@@ -49,4 +41,5 @@ Module fset.
     Qed.
   End __.
 End fset.
-Definition fset T {impls : fset.impls T} P : Type := @fset.rep T (fset.impl_with P).
+
+Definition fset T P {impl : fset.impl_with P} : Type := @fset.rep T impl.(fset._impl).
